luna attempts to implement jt

theories/codes.v
@@ -106,6 +106,83 @@ Inductive binary_tree :=
 | Empty: binary_tree
 | Node: binary_tree -> binary_tree -> binary_tree.
 
+
+(* Luna attempt at making the free jonsson tarski algeba. the node operator is usually called 
+lambda in the literature and the child operators are usually called alpha_0 alpha_1. dont know if 
+we should imitate that or stick to this. (might matter if/when we change arity) *)
+
+Inductive jt_expression :=
+| JEmpty: jt_expression
+| JNode: jt_expression -> jt_expression -> jt_expression
+| JLeft: jt_expression -> jt_expression
+| JRight: jt_expression -> jt_expression.
+
+Scheme Equality for jt_expression.
+
+
+Fixpoint jt_reduce_exp (t : jt_expression) : jt_expression :=
+  match t with
+  | JEmpty => JEmpty
+  | JNode a b => 
+      match jt_reduce_exp a, jt_reduce_exp b with
+      | JLeft x, JRight y => if (jt_expression_beq x y) then x else JNode (JLeft x) (JRight y)
+      | x, y => JNode x y
+      end
+      
+  | JLeft x =>
+      match jt_reduce_exp x with
+      | JNode a b => a
+      | y => JLeft y
+      end
+
+  | JRight x =>
+      match jt_reduce_exp x with
+      | JNode a b => b
+      | y => JRight y
+      end
+  end.
+
+Definition is_reduced_jt (t : jt_expression) : Prop := jt_reduce_exp t = t.
+
+Lemma jt_reduction_is_idempotent (t : jt_expression) : is_reduced_jt (jt_reduce_exp t).
+Proof.
+unfold is_reduced_jt.
+induction t.
+unfold jt_reduce_exp.
+reflexivity.
+Admitted.
+
+Record jt := {
+  normal_form : jt_expression;
+  is_normal_form : is_reduced_jt normal_form;
+}.
+
+Definition JTNode (l r : jt) : jt :=
+  {| normal_form :=
+       jt_reduce_exp (JNode (normal_form l) (normal_form r));
+     is_normal_form :=
+       jt_reduction_is_idempotent (JNode (normal_form l) (normal_form r));
+  |}.
+
+
+Definition JTLeft (n : jt) : jt :=
+  {| normal_form :=
+       jt_reduce_exp (JLeft (normal_form n));
+     is_normal_form :=
+       jt_reduction_is_idempotent (JLeft (normal_form n));
+  |}.
+
+Definition JTRight (n : jt) : jt :=
+  {| normal_form :=
+       jt_reduce_exp (JRight (normal_form n));
+     is_normal_form :=
+       jt_reduction_is_idempotent (JRight (normal_form n));
+  |}.
+
+Definition JTeq (x : jt) (y : jt) : bool := jt_expression_beq (normal_form x) (normal_form y).
+
+
+
 Definition Leaf := Node Empty Empty.
 Definition Caret := Node Leaf Leaf.
 
